veric/fancy_updates.v
@@ -36,35 +36,13 @@ Proof.
     iIntros "!> !>". by iApply "HP".
   - rewrite ouPred_fupd_unseal /ouPred_fupd_def. by iIntros (????) "[HwP $]".
 Qed.
-Global Instance ouPred_bi_fupd `{!wsatGS Σ} : BiFUpd (ouPredI (iResUR Σ)) :=
+Global Instance ouPred_bi_fupd `{!wsatGS Σ} : BiFUpd (iProp Σ) :=
   {| bi_fupd_mixin := ouPred_fupd_mixin |}.
 
-Global Instance ouPred_bi_bupd_fupd `{!wsatGS Σ} : BiBUpdFUpd (ouPredI (iResUR Σ)).
+Global Instance ouPred_bi_bupd_fupd `{!wsatGS Σ} : BiBUpdFUpd (iProp Σ).
 Proof. rewrite /BiBUpdFUpd ouPred_fupd_unseal. by iIntros (E P) ">? [$ $] !> !>". Qed.
 
-(*Global Instance ouPred_bi_fupd_plainly `{!wsatGS Σ} : BiFUpdPlainly (ouPredI (iResUR Σ)).
-Proof.
-  split.
-  - rewrite ouPred_fupd_unseal /ouPred_fupd_def. iIntros (E P) "H [Hw HE]".
-    iAssert (◇ ■ P)%I as "#>HP".
-    { by iMod ("H" with "[$]") as "(_ & _ & HP)". }
-    by iFrame.
-  - rewrite ouPred_fupd_unseal /ouPred_fupd_def. iIntros (E P Q) "[H HQ] [Hw HE]".
-    iAssert (◇ ■ P)%I as "#>HP".
-    { by iMod ("H" with "HQ [$]") as "(_ & _ & HP)". }
-    by iFrame.
-  - rewrite ouPred_fupd_unseal /ouPred_fupd_def. iIntros (E P) "H [Hw HE]".
-    iAssert (▷ ◇ ■ P)%I as "#HP".
-    { iNext. by iMod ("H" with "[$]") as "(_ & _ & HP)". }
-    iFrame. iIntros "!> !> !>". by iMod "HP".
-  - rewrite ouPred_fupd_unseal /ouPred_fupd_def. iIntros (E A Φ) "HΦ [Hw HE]".
-    iAssert (◇ ■ ∀ x : A, Φ x)%I as "#>HP".
-    { iIntros (x). by iMod ("HΦ" with "[$Hw $HE]") as "(_&_&?)". }
-    by iFrame.
-Qed.*)
-
-(* What's the linear equivalent of this?
-Lemma fupd_plain_soundness `{!invGpreS Σ} E1 E2 (P: iProp Σ) `{!Plain P} :
+Lemma fupd_plain_soundness `{!wsatGpreS Σ} E1 E2 (P: iProp Σ) `{!Plain P} `{!Absorbing P}:
   (∀ `{Hinv: !wsatGS Σ}, ⊢ |={E1,E2}=> P) → ⊢ P.
 Proof.
   iIntros (Hfupd). apply later_soundness. apply bupd_plain_soundness; first by apply later_plain.
@@ -74,24 +52,88 @@ Proof.
   rewrite ownE_op; last by set_solver.
   iDestruct "HE" as "[HE1 HE]".
   rewrite ouPred_fupd_unseal /ouPred_fupd_def.
-  iMod ("H" with "[$]") as "[Hw [HE2 >H']]"; iFrame.
+  iMod ("H" with "[$]") as "[Hw [HE2 >H']]"; by iFrame.
 Qed.
 
-Lemma step_fupdN_soundness `{!invGpreS Σ} φ n :
+(* an alternative to using BiFUpdPlainly, which doesn't hold in linear logics *)
+Section fupd_plain.
+
+Context `{!wsatGS Σ}.
+Implicit Types (P : iProp Σ).
+
+Lemma bupd_plainly P `{!Absorbing P}: (|==> ■ P) ⊢ P.
+Proof.
+  rewrite -{2}(absorbing P).
+  rewrite /bi_absorbingly; ouPred.unseal; split => n x Hnx /= Hng.
+  destruct (Hng n ε) as [? [_ Hng']]; try rewrite right_id; auto.
+  eexists _, _; split; last by split; [apply I | apply Hng'].
+  rewrite right_id //.
+Qed.
+
+Lemma fupd_plainly_mask_empty E `{!Absorbing P}: (|={E,∅}=> ■ P) ⊢ |={E}=> P.
+Proof.
+  rewrite -{2}(absorbing P).
+  rewrite ouPred_fupd_unseal /ouPred_fupd_def. iIntros "H [Hw HE]".
+  iAssert (◇ ■ P)%I as "#>HP".
+  { iApply bupd_plainly. iMod ("H" with "[$]") as "(_ & _ & #HP)".
+    by iIntros "!> !>". }
+  by iFrame.
+Qed.
+
+Lemma fupd_plainly_mask E E' P `{!Absorbing P}: (|={E,E'}=> ■ P) ⊢ |={E}=> P.
+Proof.
+  rewrite -(fupd_plainly_mask_empty).
+  apply fupd_elim, (fupd_mask_intro_discard _ _ _). set_solver.
+Qed.
+
+Lemma fupd_plain_mask E E' P `{!Plain P} `{!Absorbing P}: (|={E,E'}=> P) ⊢ |={E}=> P.
+Proof. by rewrite {1}(plain P) fupd_plainly_mask. Qed.
+
+Lemma fupd_plainly_later E P `{!Absorbing P}: (▷ |={E}=> ■ P) ⊢ |={E}=> ▷ ◇ P.
+Proof.
+  rewrite ouPred_fupd_unseal /ouPred_fupd_def. iIntros "H [Hw HE]".
+  iAssert (▷ ◇ ■ P)%I as "#HP".
+  { iNext. iApply bupd_plainly. iMod ("H" with "[$]") as "(_ & _ & #HP)".
+    by iIntros "!> !>". }
+  iFrame. iIntros "!> !> !>". by iMod "HP".
+Qed.
+
+Lemma fupd_plain_later E P `{!Plain P} `{!Absorbing P}: (▷ |={E}=> P) ⊢ |={E}=> ▷ ◇ P.
+Proof. by rewrite {1}(plain P) fupd_plainly_later. Qed.
+
+Lemma step_fupd_plain Eo Ei P `{!Plain P} `{!Absorbing P}: (|={Eo}[Ei]▷=> P) ⊢ |={Eo}=> ▷ ◇ P.
+Proof.
+  rewrite -(fupd_plain_mask _ Ei (▷ ◇ P)).
+  apply fupd_elim. by rewrite fupd_plain_mask -fupd_plain_later.
+Qed.
+
+Lemma step_fupdN_plain Eo Ei n P `{!Plain P} `{!Absorbing P}: (|={Eo}[Ei]▷=>^n P) ⊢ |={Eo}=> ▷^n ◇ P.
+Proof.
+  induction n as [|n IH].
+  - by rewrite -fupd_intro -bi.except_0_intro.
+  - rewrite Nat.iter_succ step_fupd_fupd IH !fupd_trans step_fupd_plain.
+    apply fupd_mono. destruct n as [|n]; simpl.
+    * by rewrite bi.except_0_idemp.
+    * by rewrite bi.except_0_later.
+Qed.
+
+End fupd_plain.
+
+Lemma step_fupdN_soundness `{!wsatGpreS Σ} φ n :
   (∀ `{Hinv: !wsatGS Σ}, ⊢@{iPropI Σ} |={⊤,∅}=> |={∅}▷=>^n ⌜ φ ⌝) →
   φ.
 Proof.
   intros Hiter.
   apply (soundness (M:=iResUR Σ) _  (S n)); simpl.
-  apply (fupd_plain_soundness ⊤ ⊤ _)=> Hinv.
+  apply (fupd_plain_soundness ⊤ ∅ _)=> Hinv.
   iPoseProof (Hiter Hinv) as "H". clear Hiter.
-  iApply fupd_plainly_mask_empty. iMod "H".
+  iMod "H".
   iMod (step_fupdN_plain with "H") as "H". iModIntro.
-  rewrite -later_plainly -laterN_plainly -later_laterN laterN_later.
+  rewrite -bi.later_laterN bi.laterN_later.
   iNext. iMod "H" as %Hφ. auto.
 Qed.
 
-Lemma step_fupdN_soundness' `{!invGpreS Σ} φ n :
+Lemma step_fupdN_soundness' `{!wsatGpreS Σ} φ n :
   (∀ `{Hinv: !wsatGS Σ}, ⊢@{iPropI Σ} |={⊤}[∅]▷=>^n ⌜ φ ⌝) →
   φ.
 Proof.
@@ -100,4 +142,4 @@ Proof.
    simpl in Hiter |- *. iMod Hiter as "H". iIntros "!>!>!>".
   iMod "H". clear. iInduction n as [|n] "IH"; [by iApply fupd_mask_intro_discard|].
   simpl. iMod "H". iIntros "!>!>!>". iMod "H". by iApply "IH".
-Qed.*)
+Qed.
